### Example:
```java
int x, m0, m1, t;

void main () {
	x = read();
	m0 = 1; m1 = 1;
	if (x > 1) f();
	write (m1)
}
```
```java
void f() {
	x = x-1;
	if (x > 1)
		f();
	t = m1;
	m1 = m0 + m1;
	m0 = t;
}
```
### Problem 
- In the logic, we must be able to distinguish between the $i$-th and the $(i + 1)$-th call.
- This is $\textcolor{skyblue}{\textbf{easier}}$, if we have `logical auxiliaries` $l = l_1,\dots,l_n$ at hand to store (selected) values $\textcolor{skyblue}{\textbf{before}}$ the call $\dots$
$$\{A\}\hspace{5mm} f(); \hspace{5mm}\{B\} \hspace{5mm} where$$
$$\begin{aligned}
A &\equiv x = l \land x > 1 \land m_0 = m_1 = 1 \\
B &\equiv l > 1 \land m_1 \le 2^l \land m_0 \le 2^{l-1}
\end{aligned}$$
- Again, we start with a `global hypothesis` `H` which provides a description where both $A$ and $B$ may contain $l_i$ for each call of $f();$
$$\{A\}\hspace{5mm} f(); \hspace{5mm}\{B\}$$
- Give this `global hypothesis H` we verify for each procedure definition `void f() {ss}` that $$\{A\}\hspace{2mm} ss \hspace{2mm}\{B\}\hspace{2mm} holds.$$ ![[Pasted image 20240902143901.png]]

- We start with an assertion for the end point:
$$B \equiv l > 1 \land m_1 \le 2^l \land m_0 \le 2^{l - 1}$$
- The assertion $C$ is obtained by means of **WP[...]** and weakening $\dots$ 
$$\begin{aligned} 
&WP[t = m1; m1 = m1 + m0; m0 = t;](B)\\
&\equiv l − 1 > 0 \land m1 + m0 \le 2^l \land m1 \le 2 ^ {l−1} \\
&\Leftarrow l − 1 > 1 \land m1 \le 2^{l−1} \land m0 \leq 2^{l−2} \\
&\equiv C
\end{aligned}$$
### Question
How can the `global hypothesis be used to deal with a specific procedure call`???
- The assertion $\{A\} \hspace{2mm} f(); \hspace{2mm}\{B\}$ represents a $\textcolor{skyblue}{\textbf{value table}}$ for $f()$.
- This value table can be logically represented by the implication:
$$\forall l. \hspace{2mm} (A[h/x] \Rightarrow B)$$ // h denotes a sequence of $\textcolor{pink}{\textbf{auxiliaries}}$.
- The values of the variables `x` before the call are recorded in the $\textcolor{pink}{\textbf{auxiliaries}}$ 
### Examples
- Function: $\hspace{5mm}\text{void double () { x = 2*x;}}$
- Specification: $\hspace{5mm} \text{\{x = l\} double(); \{x = 2l\}}$ 
- Table: $\hspace{5mm} \forall l.(h = l) \Rightarrow (x = 2l) \equiv (x = 2h)$

- For the Fibonnaci function, we calculate:
$$\begin{aligned}
\forall l. (h > 1 \land h = l \land h_0 = h_1 = 1)\\ &\Rightarrow l > 1 \land m_1 \le 2^l \land m_0 \le 2^{l-1} \\
&\equiv (h > 1 \land h_0 = h_1 = 1) \\ &\Rightarrow m_1 \le 2^h \land m_0 \le 2^{h−1}
\end{aligned}$$
- Another pair $(A_1, B_1)$ of assertions forms a valid triple $\{A_1\}\hspace{2mm}f();\hspace{2mm}\{B_1\}$, if we are able to prove that $$\frac{\forall l. A[h/x]\Rightarrow B \hspace{10mm}A_1[h/x]}{B_1}$$
**Example** double()$$\begin{aligned} A &\equiv x = l && B \equiv x = 2l \\
								 A_1 &\equiv x \ge 3 && B_1 \equiv x \ge 6 
\end{aligned}$$
We verify: $$\frac{x = 2h \hspace{10mm} h \ge 3}{x\ge 6}$$
Valid pairs $(A_1, B _1)$ are obtained:
- by $\textcolor{skyblue}{\textbf{substituting}}$ logical variables:$$\frac{\{x = l\} \hspace{2mm} double(); \hspace{2mm}\{x = 2l\}}{\{x = l -1\}\hspace{2mm} double(); \hspace{2mm} \{x = 2(l -1)\}}$$
- by adding a condition $C$ to the logical variables: $$\frac{\{x = l\} \hspace{2mm} double(); \hspace{2mm}\{x = 2l\}}{\{x = l \land l > 0\}\hspace{2mm} double(); \hspace{2mm} \{x = 2l \land l > 0\}}$$
Valid pairs $(A_1, B _1)$ are also obtained:
- if the `pre-condition` is $\textcolor{skyblue}{\textbf{strengthened}}$ or the `post-condition` $\textcolor{skyblue}{\textbf{weakened}}$:$$
\frac{\{x = l\} \hspace{2mm} double(); \hspace{2mm}\{x = 2l\}}{\{x > 0 \land x = l \}\hspace{2mm} double(); \hspace{2mm} \{x = 2l \lor x = -1 \}} $$$$
\frac{\{x = l\} \hspace{2mm} double(); \hspace{2mm}\{x = 2l\}}{\{x = l \}\hspace{2mm} double(); \hspace{2mm} \{x = 2l \lor x = -1 \}} $$

# Links: 




202409021402
[[2024-09-02]]