- ![[Drawing 2024-09-01 18.38.59.excalidraw]]
- *It should hold:* 
$$\begin{aligned} &A \land \neg b \Rightarrow B_0 \hspace{2mm}and \\ &A \land b \Rightarrow B_1 \end{aligned}$$
- This is the case, if A implies the weakest pre-condition of the conditional branching: 
$$WP[b](B_0,B_1) \equiv ((\neg b) \Rightarrow B_0) \land (b \Rightarrow B_1)$$
- The weakest pre-condition can be rewritten into:
$$\begin{aligned}WP[b](B_0, B_1) &\equiv (b \lor B_0) \land (\neg b \lor B_1) \\ &\equiv (\neg b \land B_0) \lor (b \land B_1) \lor (B_0 \land B_1) \\ &\equiv (\neg b \land B_0) \lor (b \land B_1)\end{aligned}$$
#### Example:
$$B_0 \equiv x > y \hspace{2mm} \land \hspace{2mm}y > 0 \hspace{15mm}B_0 \equiv y > x \hspace{2mm} \land \hspace{2mm}x > 0$$
- Assume that `b` is the condition `y > x`.
- Then the weakest pre-condition is given by:
$$\begin{aligned}&(x \ge y \land x > y \land y > 0) \lor (y > x \land y > x \land 0) \\ &\equiv (x > y \land y > 0) \lor (y > x \land x > 0) \\ &\equiv x > 0 \land y > 0 \land x \neq y \end{aligned}$$

# Links: 




202409011839
[[2024-09-01]]