### Orientation![[Pasted image 20240902152722.png]]

Our goal is to prove: $\{D\}\hspace{2mm}f();\hspace{2mm}\{C\}$
$$\begin{aligned}
&A &&\equiv x > 1 \land l = x \land m_0 = m_1 = 1 \\
&A[(l - 1)/l] &&\equiv x > 1 \land l - 1 = x \land m_0 = m_1 = 1 \\
&&&\equiv D
\end{aligned}$$
$$\begin{aligned}
&A &&\equiv l > 1 \land m_1 \le 2^l \land m_0 \le 2^{l-1} \\
&B[(l - 1)/l] &&\equiv l - 1 > 1 \land m_1 \le 2^{l-1} \land m_0 \le 2^{l-2} \\
&&&\equiv C
\end{aligned}$$
$\textcolor{green}{\textbf{For the conditional we, verify:}}$ $$\begin{aligned}
WP[x > 1](B, D) &\equiv (x \le 1 \land l > 1 \land m_1 \le 2^l \land m_0 \le 2^{l−1}) \lor \\&(x > 1 \land x = l − 1 \land m_1 = m_0 = 1) \\
&\Leftarrow x > 0 \land x = l − 1 \land m_0 = m_1 = 1
\end{aligned}$$

# Links: 




202409021526
[[2024-09-02]]